checkpoint

Vizing/new/Fan.lean
@@ -34,6 +34,7 @@ structure Fan (x y : Vertex n) where
   nonemptyAx : val ≠ #[]
   firstElemAx : val[0]'(by exact Array.size_pos_iff.mpr nonemptyAx) = y
   colorAx : colorAx n c G C val x
+  nodupAx : val.toList.Nodup
 
 def default (x y : Vertex n) (h : present n G (x, y)) : Fan n c G C x y where
   val := #[y]
@@ -43,17 +44,105 @@ def default (x y : Vertex n) (h : present n G (x, y)) : Fan n c G C x y where
   firstElemAx := by congr
   nonemptyAx := by exact Array.ne_empty_of_size_eq_add_one rfl
   colorAx := by simp [colorAx]
+  nodupAx := by simp
 
-def add (x y : Vertex n) (F : Array (Vertex n))
-  (nbors : List (Vertex n)) (h : F ≠ #[]) : Array (Vertex n) :=
+def add (x y : Vertex n) (F : Array (Vertex n)) (nbors : List (Vertex n))
+  (h : F ≠ #[]) :=
+  match (List.attach nbors).find? (fun ⟨z, _⟩ ↦
+    color n c G C (x, z) ∈ freeColorsOn n c G C (F.back (Array.size_pos_iff.mpr h))) with
+  | some z => add x y (F.push z.val) (nbors.erase z.val) Array.push_ne_empty
+  | none => F
+  termination_by nbors.length
+  decreasing_by
+    rw [List.length_erase_of_mem z.prop]
+    apply Nat.sub_one_lt_of_le
+    apply List.length_pos_iff_exists_mem.mpr
+    exact ⟨z.val, z.prop⟩
+    rfl
+
+theorem add_nborsAx (x y : Vertex n) (F : Array (Vertex n))
+  (nbors : List (Vertex n)) (hne : F ≠ #[]) (h : F.toList ⊆ nbhd n G x)
+  (hn : nbors ⊆ nbhd n G x) :
+  (add n c G C x y F nbors hne).toList ⊆ nbhd n G x := by
+  induction F, nbors, hne using add.induct n c G C x
+  · rename_i F nbors hne z hz ih
+    rw [add]; simp_all
+    apply ih
+    · exact hn z.prop
+    · grw [List.erase_subset]; assumption
+  · rename_i nbors _ _ hz
+    rw [add, hz]; simp_all
+
+theorem add_nonemptyAx (x y : Vertex n) (F : Array (Vertex n))
+  (nbors : List (Vertex n)) (hne : F ≠ #[]) :
+  (add n c G C x y F nbors hne) ≠ #[] := by
+  induction F, nbors, hne using add.induct n c G C x
+  · rw [add]; simp_all
+  · rename_i hz
+    rw [add, hz]; simp_all
+
+theorem add_firstElemAx (x y : Vertex n) (F : Array (Vertex n))
+  (nbors : List (Vertex n)) (hne : F ≠ #[])
+  (h : F[0]'(Array.size_pos_iff.mpr hne) = y) :
+  (add n c G C x y F nbors hne)[0]'(Array.size_pos_iff.mpr
+    (add_nonemptyAx n c G C x y F nbors hne)) = y := by
+  induction F, nbors, hne using add.induct n c G C x
+  · rename_i F nbors hne z hz ih
+    unfold add; simp_all only
+    apply ih
+    simp_all [Array.getElem_push]
+  · unfold add; simp_all only
+
+theorem add_colorAx (x y : Vertex n) (F : Array (Vertex n))
+  (nbors : List (Vertex n)) (hne : F ≠ #[]) (h : colorAx n c G C F x) :
+  colorAx n c G C (add n c G C x y F nbors hne) x := by
+  simp [colorAx]
+  induction F, nbors, hne using add.induct n c G C x
+  · rename_i F nbors hne z hz ih
+    rw [add]; simp_all only
+    apply ih
+    simp [colorAx] at ⊢ h
+    intro i hi
+    by_cases hsize : i < F.size - 1
+    · have : (F.push z)[i+1]'(by simp [Array.size_push]; linarith) = F[i+1] := by
+        apply Array.getElem_push_lt
+      simp [Array.getElem_push_lt hi, this]
+      exact h i hsize
+    · have : i = F.size - 1 := by
+        simp at hsize; omega
+      subst this
+      simp [Nat.sub_add_cancel (Nat.one_le_of_lt hi), Array.getElem_push_lt hi]
+      apply List.find?_some at hz; simp [Array.back] at hz
+      exact hz
+  · rw [add]
+    simp_all only [colorAx, implies_true]
+
+
+
+
+
+
+
+
+
+
+
+
+
+
+#exit
+
+def add_next (x y : Vertex n) (F : Array (Vertex n))
+  (nbors : List (Vertex n)) (h : F ≠ #[]) : Array (Vertex n) × List (Vertex n) :=
   match nbors with
-  | [] => F
+  | [] => (F, [])
   | next :: rest =>
     if color n c G C (x, next) ∈ freeColorsOn n c G C
       (F.back (by exact Array.size_pos_iff.mpr h)) then
-    add x y (F.push next) rest (by exact Array.push_ne_empty) else
-    add x y F rest h
+      ((F.push next), rest) else
+    Prod.map id (next :: ·) (add_next x y F rest h)
 
+#exit
 theorem add_nborsAx (x y : Vertex n) (F : Array (Vertex n))
   (nbors : List (Vertex n)) (hne : F ≠ #[]) (h : F.toList ⊆ nbhd n G x)
   (hn : nbors ⊆ nbhd n G x) :
@@ -125,6 +214,43 @@ theorem add_colorAx (x y : Vertex n) (F : Array (Vertex n))
       assumption
   · exact ih F hne h
 
+theorem add_nodupAx (x y : Vertex n) (F : Array (Vertex n))
+  (nbors : List (Vertex n)) (hn : nbors.Nodup) (hne : F ≠ #[]) (h : F.toList.Nodup)
+  (hdisjoint : List.Disjoint nbors F.toList) :
+  (add n c G C x y F nbors hne).toList.Nodup := by
+  induction' nbors with z zs ih generalizing F
+  <;> simp [add]
+  · assumption
+  split_ifs; all_goals rename_i h'
+  · apply ih
+    · exact List.Nodup.of_cons hn
+    · simp only [Array.toList_push]
+      apply List.nodup_append.mpr
+      repeat any_goals apply And.intro
+      · assumption
+      · exact List.nodup_singleton z
+      · exact List.Disjoint.symm
+          (List.disjoint_of_disjoint_append_left_left hdisjoint)
+    · simp only [Array.toList_push]
+      apply List.disjoint_append_right.mpr
+      constructor
+      · exact List.Disjoint.symm (List.disjoint_of_disjoint_cons_right
+        (List.Disjoint.symm hdisjoint))
+      · exact List.Disjoint.symm (List.disjoint_of_nodup_append hn)
+  · apply ih
+    · exact List.Nodup.of_cons hn
+    · assumption
+    · exact List.Disjoint.symm (List.disjoint_of_disjoint_cons_right
+      (List.Disjoint.symm hdisjoint))
+
+theorem add_is_maximal (x y : Vertex n) (F : Array (Vertex n))
+  (nbors : List (Vertex n)) (hn : nbors.Nodup) (hne : F ≠ #[]) :
+  ¬ ∃ v, ((add n c G C x y F nbors hne).push v).toList.Nodup ∧
+    colorAx n c G C ((add n c G C x y F nbors hne).push v) x := by
+
+  sorry
+
+
 def mkMaxFan (x y : Vertex n) (h : present n G (x, y)) : Array (Vertex n) :=
   add n c G C x y (default n c G C x y h).val
   ((nbhd n G x).val.erase y) (default n c G C x y h).nonemptyAx
@@ -154,11 +280,23 @@ theorem mkMaxFan_colorAx (x y : Vertex n) (hpres : present n G (x, y)) :
   colorAx n c G C (mkMaxFan n c G C x y hpres) x := by
   simp [mkMaxFan, (default n c G C x y hpres).colorAx, add_colorAx]
 
+theorem mkMaxFan_nodupAx (x y : Vertex n) (hpres : present n G (x, y)) :
+  (mkMaxFan n c G C x y hpres).toList.Nodup := by
+  simp [mkMaxFan, default]
+  apply add_nodupAx
+  · apply List.Nodup.erase y
+    exact (nbhd n G x).prop.right
+  · exact List.nodup_singleton y
+  · apply List.disjoint_singleton.mpr
+    apply List.Nodup.not_mem_erase
+    exact (nbhd n G x).prop.right
+
 def maximalFan (x y : Vertex n) (h : present n G (x, y)) : Fan n c G C x y where
   val := mkMaxFan n c G C x y h
   nborsAx := mkMaxFan_nborsAx n c G C x y h
   firstElemAx := mkMaxFan_firstElemAx n c G C x y h
   nonemptyAx := mkMaxFan_nonemptyAx n c G C x y h
   colorAx := mkMaxFan_colorAx n c G C x y h
+  nodupAx := mkMaxFan_nodupAx n c G C x y h
 
 end Fan
